src/tls/Negotiation.fsti
@@ -1,0 +1,350 @@
+module Negotiation
+
+/// Negotiates the TLS parameters for connection establishment, based
+/// on the local configuration and the peer's hello message.
+///
+/// Defines datatypes holding the TLS parameters: [offer] and [mode]
+/// used in Handshake, FFI, QUIC.
+
+// application-specific negotation relies on a callback in the
+// configuration.
+
+open FStar.Error
+open FStar.Bytes
+
+open Mem
+open TLSError
+open TLSInfo
+open TLSConstants
+open HandshakeMessages
+
+module HS = FStar.HyperStack
+module HST = FStar.HyperStack.ST
+
+/// What's an appropriate abstraction? Provide both pure specs and the
+/// supporting state machine? Keep offer and mode transparent?
+
+type share = g:CommonDH.group & CommonDH.share g
+type pre_share = g:CommonDH.group & CommonDH.pre_share g
+
+let offer = HandshakeMessages.ch 
+
+(*
+  We keep both the server's HelloRetryRequest
+  and the overwritten parts of the initial offer
+*)
+type retryInfo (offer:offer) =
+  hrr *
+  list pre_share (* we should actually keep the raw client extension content *) *
+  list Extensions.pskIdentity
+
+val find_cookie: offer -> option (b:bytes {0 < length b /\ length b < 65536})
+val find_psk_key_exchange_modes: offer -> list Extensions.psk_kex // [] when not found; pick better representation?
+val find_sessionTicket: offer -> option bytes // TODO refine
+val find_clientPske: offer -> 
+  option (
+    identities: list Extensions.pskIdentity {let n = length (Extensions.pskiListBytes identities) in 6 < n /\ n < 65536} * 
+    binders_len: nat {binders_len <= 65535})
+
+type pski (o:offer) = n:nat {
+  // o.ch_protocol_version = TLS_1p3 /\ // 19-01-04  was mistaken?
+  (match find_clientPske o with
+  | Some (ids,_) -> n < List.length ids
+  | _ -> False) }
+
+(*
+  The final negotiated outcome, including key shares and long-term identities.
+  mode is the name used in the resilience paper;
+  session_info is the one from TLSInfo
+*)
+// can we make it abstract? get rid of accessor functions? used directly in Handshake. 
+noeq type mode =
+  | Mode:
+    n_offer: offer -> // negotiated client offer
+    n_hrr: option (retryInfo n_offer) ->  // optional HRR roundtrip
+
+    // more from SH (both TLS 1.2 and TLS 1.3)
+    n_protocol_version: protocolVersion ->
+    n_server_random: TLSInfo.random ->
+    n_sessionID: sessionID ->
+    n_cipher_suite: cipherSuite ->
+
+    // redundant with the server extension response?
+    n_pski: option (pski n_offer) -> // only for TLS 1.3, result of a tricky stateful computation
+
+    // concatenating SH and EE extensions for 1.3, in wire order
+    // 18-09-09 recheck we exclude ambiguity
+    n_server_extensions: option (se:list Extensions.extension{List.Tot.length se < 256}) ->
+
+    // more from SKE in ...ServerHelloDone (1.2) or SH (1.3)
+    n_server_share: option share ->
+
+    // more from either ...ServerHelloDone (1.2) or ServerFinished (1.3)
+    n_client_cert_request: option HandshakeMessages.cr ->
+    n_server_cert: option (Cert.chain13 * signatureScheme) ->
+
+    // more from either CH+SH (1.3) or CKE (1.2)
+    n_client_share: option share ->
+    // { both shares are in the same negotiated group }
+    mode
+
+type resumeInfo =
+  option (psk_identifier * t:Ticket.ticket{Ticket.Ticket12? t}) *
+  list (psk_identifier * t:Ticket.ticket{Ticket.Ticket13? t})
+
+// main negotation state (why are we duplicating the nonce? to make it clearly stateless?)
+// 19-01-06 how to declare an opaque noeq?
+
+type certNego = option (cert_type * signatureScheme)
+
+val find_early_data: offer -> option Extensions.earlyDataIndication 
+
+
+noeq type negotiationState (r:role) (cfg:config) : Type0 =
+  // Have C_Offer_13 and C_Offer? Shares aren't available in C_Offer yet
+  | C_Init:     n_client_random: TLSInfo.random ->
+                negotiationState r cfg
+
+  | C_Offer:    n_offer: offer ->
+                negotiationState r cfg
+
+  | C_HRR:      n_offer: offer ->
+                n_hrr: retryInfo n_offer ->
+                negotiationState r cfg
+
+  | C_WaitFinished1:
+                n_partialmode: mode ->
+                negotiationState r cfg
+
+  | C_Mode:     n_mode: mode -> // In 1.2, used for resumption and full handshakes
+                negotiationState r cfg
+
+  | C_WaitFinished2: // Only 1.2
+                n_mode: mode ->
+                n_client_certificate: option Cert.chain13 ->
+                negotiationState r cfg
+
+  | C_Complete: n_mode: mode ->
+                n_client_certificate: option Cert.chain13 ->
+                negotiationState r cfg
+
+  | S_Init:     n_server_random: TLSInfo.random ->
+                negotiationState r cfg
+
+  // Waiting for ClientHello2
+  | S_HRR:      n_offer: offer ->
+                n_hrr: hrr ->
+                negotiationState r cfg
+
+  | S_ClientHello: // Transitional state to allow Handshake to call KS and generate a share
+                n_mode: mode -> // n_server_share and n_server_extensions are None
+                // We ask for a certificate from the PKI library - this is just a handle
+                // If a certificate is actually used, it appears in network format in mode.n_server_cert
+                n_selected_cert: certNego ->
+                negotiationState r cfg
+
+  // This state is used to wait for both Finished1 and Finished2
+  | S_Mode:     n_mode: mode -> // If 1.2, then client_share is None
+                n_selected_cert: certNego ->
+                negotiationState r cfg
+
+  | S_Complete: n_mode: mode ->
+                n_client_certificate: option Cert.chain13 ->
+                negotiationState r cfg
+
+// assume val ns_rel_monotonic: #r:role -> #cfg:config ->
+//   Lemma (Preorder.preorder_rel (ns_rel #r #cfg))
+
+// main negotation state (why are we duplicating the nonce? to make it clearly stateless?)
+
+noeq type t (region:rgn) (role:TLSConstants.role) : Type0 =
+  | NS:
+    cfg: config -> // local configuration
+    resume: resumeInfo ->
+    nonce: TLSInfo.random ->
+    state: HST.reference (negotiationState role cfg) { HS.frameOf state = region }->
+    t region role
+
+
+val create:
+  region:rgn -> 
+  r:role -> 
+  cfg:config -> 
+  nonce: TLSInfo.random -> 
+  St (t region r)
+  // ensures ns.cfg = cfg /\ ns.nonce = nonce /\ initial state. 
+
+type reader 'a = 
+  #region:rgn -> #role:TLSConstants.role -> ns:t region role -> ST 'a 
+  (requires (fun h0 -> h0 `HS.contains` ns.state ))
+  (ensures (fun h0 _ h1 -> h0 == h1))
+
+// For QUIC, the handshake signals it is returning HRR (to issue a special packet type)
+val is_server_hrr: reader bool 
+
+val hashAlg: mode -> Hashing.Spec.alg
+val kexAlg: mode -> TLSConstants.kexAlg
+val aeAlg:
+  m:mode{CipherSuite? m.n_cipher_suite \/ CipherSuite13? m.n_cipher_suite} ->
+  TLSConstants.aeAlg
+val emsFlag: mode -> bool
+
+// used only for TLS 1.2. FIXME: properly negotiate
+val chosenGroup: m:mode {
+  match kexAlg m with 
+  | Kex_PSK_DHE
+  | Kex_DHE 
+  | Kex_PSK_ECDHE
+  | Kex_ECDHE -> True 
+  | _ -> False } -> option CommonDH.group
+
+val zeroRTToffer: offer -> bool
+val zeroRTT: mode -> bool
+
+val sendticket_12: mode -> bool
+val resume_12: mode -> bool
+
+val local_config: 
+  #region:rgn -> #role:TLSConstants.role -> t region role -> 
+  Tot config
+
+val nonce: 
+  #region:rgn -> #role:TLSConstants.role -> t region role -> 
+  Tot TLSInfo.random
+
+val resume: 
+  #region:rgn -> #role:TLSConstants.role -> t region role -> 
+  Tot resumeInfo
+
+val getMode: reader mode
+
+(* Returns the negotiated version, when known, or cfg.max_version *)
+val version: reader protocolVersion 
+val is_hrr: reader bool
+
+// TODO 19-01-06 effect of signing
+val sign: 
+  #region:rgn -> #role:TLSConstants.role -> ns:t region role -> 
+  bytes -> 
+  ST (result HandshakeMessages.signature)
+  (requires (fun h0 -> h0 `HS.contains` ns.state ))
+  (ensures (fun h0 _ h1 -> h0 == h1))
+
+
+(* CLIENT *) 
+
+val client_ClientHello: 
+  #region:rgn -> t region Client -> 
+  oks: option CommonDH.clientKeyShare -> 
+  St offer
+  // [C_Init ==> C_Offer]
+  // ensures offer = client_offer ns.cfg ns.nonce oks ns.resume now [used e.g. for binder auth] 
+  // oks: optional client key shares created by ks_client_init
+  // now: stateful time for age obfuscation (return it ghostly?)
+
+val group_of_hrr: HandshakeMessages.hrr -> option CommonDH.group
+
+val client_HelloRetryRequest:
+  #region:rgn -> t region Client -> 
+  hrr -> 
+  option share -> 
+  St (result offer) 
+  // [C_Offer ==> C_HRR] TODO separate pure spec
+  
+val client_ServerHello: 
+  #region:rgn -> 
+  t region Client ->
+  HandshakeMessages.sh ->
+  St (result mode) 
+  // [C_Offer | C_HRR_offer ==> C_Mode] with TODO hrr.  
+  // ensures client_mode ns offer sh == Correct mode
+
+// used internally, but also directly called by Handshake 
+val to_be_signed: 
+  pv:protocolVersion -> 
+  role -> 
+  csr:option (lbytes 64) -> 
+  tbs:bytes {(None? csr <==> pv == TLS_1p3) /\ Bytes.length tbs <= 128} -> 
+  bytes
+
+val client_ServerKeyExchange: 
+  #region:rgn -> t region Client ->
+  serverCert:HandshakeMessages.crt ->
+  HandshakeMessages.ske ->
+  ocr:option HandshakeMessages.cr ->
+  St (result mode)
+  // [C_Mode ==> C_Mode] setting [server_share; client_cert_request; server_cert] in mode,
+  // requires mode.n_protocol_version = TLS_1p2
+
+val clientComplete_13: 
+  #region:rgn -> t region Client ->
+  ee: HandshakeMessages.ee ->
+  optCertRequest: option HandshakeMessages.cr13 ->
+  optServerCert: option Cert.chain13 -> // Not sent with PSK
+  optCertVerify: option HandshakeMessages.cv -> // Not sent with PSK
+  digest: option (b:bytes{length b <= 32}) ->
+  St (result mode) // it needs to be computed, whether returned or not
+  // [C_Mode ==> C_Complete] setting [sexts optCertRequest schain] in mode and recording [ccert]
+  // ensures schain-based server authentication of the mode (including sexts) 
+  // ensures consistency of sexts and schain with the offer.
+  // TODO client sigs; till then ccert=None and optCertRequest is ignored.
+
+
+(* SERVER *) 
+
+// For application-handled extensions set by nego callback,
+// such as QUIC transport parameters
+type extra_ext = list Extensions.extension // to be refined 
+
+//17-03-30 still missing a few for servers.
+noeq type serverMode =
+  | ServerHelloRetryRequest: hrr:hrr ->
+    cs:cipherSuite{name_of_cipherSuite cs = hrr.hrr_cipher_suite} ->
+    serverMode
+  | ServerMode: mode -> certNego -> extra_ext -> serverMode
+
+(* Returns the server name, if any, or an empty bytestring; review. *)
+val get_sni: offer -> Tot bytes 
+
+(* for QUIC *) 
+val get_alpn: offer -> Tot alpn
+
+val server_ClientHello: 
+  #region:rgn -> t region Server ->
+  HandshakeMessages.ch -> 
+  log:HandshakeLog.t ->
+  St (result serverMode)
+  // [S_Init | S_HRR ==> S_ClientHello m cert] 
+  // ensures r = computeServerMode ns.cfg ns.nonce offer (stateful)
+  // but [compute_cs13] and [negotiateCipherSuite] are pure. 
+
+/// Complete the server's mode with its DH share
+/// (the two-step decomposition enables DH generation from partial mode in-between)
+/// 
+val server_ServerShare: 
+  #region:rgn -> 
+  t region Server ->
+  oks:option CommonDH.serverKeyShare -> 
+  app_exts: extra_ext ->
+  St (result mode)
+  // [S_ClientHello ==> S_Mode] setting [sexts, oks] in mode
+  // requires oks is consistent with mode (?)
+  // ensures sexts = server_negotiateExtensions ns mode cexts @ app_exts
+  // review their ordering, and how QD separates them
+
+
+//17-03-30 get rid of this wrapper?
+noeq type session = {
+  session_nego: option mode;
+}
+
+// represents the outcome of a successful handshake,
+// providing context for the derived epoch
+noeq type handshake =
+  | Fresh of session // was sessionInfo
+  | Resumed of session // was abbrInfo * sessionInfo
+// We use SessionInfo as unique session indexes.
+// We tried using instead hs, but this creates circularities
+// We'll probably need a global log to reason about them.
+// We should probably do the same in the session store.
+
